ocamllibs/dafny_examples/Example_is_sorted.dfy
@@ -1,21 +1,34 @@
 function DfLength(s: seq<int>): int
 {if s == [] then 0 else DfLength(s[..|s|-1]) + 1}
 
+function DfMin(x: int, y: int): int { if x > y then y else x}
+
+function DfMinSeq(s : seq<int>) : int 
+  requires |s| >= 1
+{
+  if |s| == 1 then s[0]
+  else
+  DfMin(DfMinSeq(s[..|s|-1]), s[|s|-1])
+}
 function Aux_0(a : seq<int>): int
 requires |a| >= 1
-{ if |a| == 1 then  a[0] else  a[0] 
+{
+  if |a| == 1 then a[0] else a[0]
 }
 
 function Iss(a : seq<int>): bool
-{ if a == [] then
+requires |a| >= 1
+{
+  if |a| == 1 then
     true
-   else 
-   (Iss(a[..|a|-1]) && (Prev(a[..|a|-1]) < a[|a|-1]))
-   
+    else
+    (Iss(a[..|a|-1]) && (Prev(a[..|a|-1]) < a[|a|-1]))
 }
 
 function Prev(a : seq<int>): int
-{ if a == [] then  0 else  a[|a|-1] 
+requires |a| >= 1
+{
+  if |a| == 1 then a[0] else a[|a|-1]
 }
 
 function Aux_0Join(leftAux_0 : int, rightAux_0 : int): int
@@ -25,7 +38,7 @@ function Aux_0Join(leftAux_0 : int, rightAux_0 : int): int
 
 function IssJoin(leftAux_0 : int, leftPrev : int, leftIss : bool, rightAux_0 : int, rightPrev : int, rightIss : bool): bool
 {
-  (((rightAux_0 - leftPrev) > ((-1) + 1)) && (rightIss && leftIss))
+  (((rightAux_0 - leftPrev) >= 1) && (leftIss && rightIss))
 }
 
 function PrevJoin(leftPrev : int, rightPrev : int): int
@@ -35,6 +48,7 @@ function PrevJoin(leftPrev : int, rightPrev : int): int
 
 
 lemma HomAux_0(a : seq<int>, R_a : seq<int>)
+  requires |a| >= 1 && |R_a| >= 1
   ensures Aux_0(a + R_a) == Aux_0Join(Aux_0(a), Aux_0(R_a))
   {
     if |R_a| == 1 
@@ -51,15 +65,17 @@ lemma HomAux_0(a : seq<int>, R_a : seq<int>)
 } // End lemma.
 
 lemma BaseCaseIss(a : seq<int>, R_a : seq<int>)
-  ensures Iss(a) == IssJoin(Aux_0(a), Prev(a), Iss(a), Aux_0([R_a[0]]), Prev([R_a[0]]), Iss([R_a[0]]))
+  requires |a| >= 1 && |R_a| >= 1
+  ensures Iss(a + [R_a[0]]) == IssJoin(Aux_0(a), Prev(a), Iss(a), Aux_0([R_a[0]]), Prev([R_a[0]]), Iss([R_a[0]]))
   {}
 
 lemma HomIss(a : seq<int>, R_a : seq<int>)
+  requires |a| >= 1 && |R_a| >= 1
   ensures Iss(a + R_a) == IssJoin(Aux_0(a), Prev(a), Iss(a), Aux_0(R_a), Prev(R_a), Iss(R_a))
   {
-    if R_a == [] 
+    if |R_a| == 1 
     {
-    assert(a + [] == a);
+    assert(a + R_a == a + [R_a[0]]);
     BaseCaseIss(a, R_a);
     
      } else {
@@ -75,17 +91,19 @@ lemma HomIss(a : seq<int>, R_a : seq<int>)
   } // End else.
 } // End lemma.
 
-lemma BaseCasePrev(a : seq<int>)
-  ensures Prev(a) == PrevJoin(Prev(a), Prev([]))
+lemma BaseCasePrev(a : seq<int>, R_a : seq<int>)
+  requires |a| >= 1 && |R_a| >= 1
+  ensures Prev(a + [R_a[0]]) == PrevJoin(Prev(a), Prev([R_a[0]]))
   {}
 
 lemma HomPrev(a : seq<int>, R_a : seq<int>)
+  requires |a| >= 1 && |R_a| >= 1
   ensures Prev(a + R_a) == PrevJoin(Prev(a), Prev(R_a))
   {
-    if R_a == [] 
+    if |R_a| == 1 
     {
-    assert(a + [] == a);
-    BaseCasePrev(a);
+    assert(a + R_a == a + [R_a[0]]);
+    BaseCasePrev(a, R_a);
     
      } else {
     calc{
